src/Verify.v
@@ -19,179 +19,90 @@ Section Verify.
 Variable maxReg : nat.          (* max number of registers *)
 Definition PhysReg := 'I_maxReg.
 
-Variable maxVar : nat.          (* max number of variables *)
-Hypothesis variables_exist : 0 < maxVar.
-
 Variables opType1 opType2 : Set.
 Variables mType : Type -> Type.
 Context `{mDict : Monad mType}.
 
 Variable oinfo : OpInfo maxReg opType1 opType2.
 
-Inductive UseVerifier :=
-  | VerifyDisabled
-  | VerifyEnabledUnitializedOK
-  | VerifyEnabled.
+Inductive UseVerifier := VerifyDisabled | VerifyEnabled.
+
+Definition RegAllocations := Vec (option VarId * option VarId) maxReg.
 
 Record RegStateDesc := {
-  rsRegs        : Vec (option 'I_maxVar) maxReg;
-  rsAllocs      : Vec (option 'I_maxReg) maxVar;
-  rsGhostRegs   : Vec (option 'I_maxVar) maxReg;
-  rsGhostAllocs : Vec (option 'I_maxReg) maxVar;
-  rsStack       : Vec bool maxVar
+  rsAllocs : RegAllocations;
+  rsStack  : IntSet
 }.
 
+Definition residency :
+  Lens' (option VarId * option VarId) (option VarId) := _1.
+Definition reservation :
+  Lens' (option VarId * option VarId) (option VarId) := _2.
+
 Definition newRegStateDesc : RegStateDesc :=
-  {| rsRegs        := vconst None
-   ; rsAllocs      := vconst None
-   ; rsGhostRegs   := vconst None
-   ; rsGhostAllocs := vconst None
-   ; rsStack       := vconst false
+  {| rsAllocs := vconst (None, None)
+   ; rsStack  := emptyIntSet
    |}.
-
-Definition IntSet_to_seq_fin {n : nat} (s : IntSet) :
-  all (ltn ^~ n) (IntSet_toList s) -> seq 'I_n.
-Proof.
-  elim: (IntSet_toList s) => [_|? ? IHxs /andP [H ?]] /=.
-    exact: [::].
-  exact: cons (Ordinal H) (IHxs _).
-Defined.
-
-Definition keepOnly {A : Type} `(xs : seq 'I_n) :
-  Vec (option A) n -> Vec (option A) n :=
-  vmap_with_index (fun i x => if i \in xs then x else None).
 
 (* The pattern is: actual, actual, expected *)
 Inductive AllocError :=
-  | VarId_OutOfBounds of VarId & nat
   | VarNotAllocated of VarId
-  | FreeUnallocatedVar of VarId
-  | FreeVarAllocatedToDifferentReg of VarId & nat & nat
-  | FreeRegNotAllocatedToVar of nat & VarId
-  | VarWithoutAllocation of VarId
-  | AllocVarAllocatedToDifferentReg of VarId & nat & nat
-  | CheckVarAllocatedToDifferentReg of VarId & nat & nat
-  | MoveRegNotAllocated of nat & nat
-  | SwapRegNotAllocated of nat & nat
-  | SpillRegNotAllocated of nat & nat
-  | RegNotAllocatedToVar of nat & VarId
-  | CheckRegAllocatedToDifferentVar of nat & VarId & VarId
-  | AllocRegAllocatedToDifferentVar of nat & VarId & VarId
-  | RegAlreadyAllocatedTo of nat & VarId
-  | SpillToWrongSlot of nat & VarId & VarId
+  | VarNotResident of VarId
+  | VarNotResidentForReg of VarId & nat
+  | VarNotReservedForReg of VarId & nat
+  | PhysRegAlreadyResidentForVar of nat & VarId
+  | PhysRegAlreadyReservedForVar of nat & VarId
+  | RegAlreadyReservedToVar of nat & VarId & VarId
   | BlockWithoutPredecessors of BlockId
   | UnknownPredecessorBlock of BlockId & BlockId
   | ErrorAtBlockEnd of BlockId.
 
-Definition checkAlloc' st (var : 'I_maxVar) (mreg : option 'I_maxReg)
-  (strict : bool) (checkGhosts : bool) :
-  option AllocError :=
-  let check regs reg :=
-    let res :=
-      if vnth regs reg isn't Some var'
-      then Some (RegNotAllocatedToVar reg var)
-      else
-        if var == var'
-        then None
-        else Some (CheckRegAllocatedToDifferentVar reg var' var) in
-    if mreg is Some reg'
-    then if reg == reg'
-         then res
-         else Some (CheckVarAllocatedToDifferentReg var reg reg')
-    else res in
-  let go :=
-    if vnth (rsAllocs st) var is Some reg
-    then check (rsRegs st) reg
-    else
-      if strict
-      then Some (VarNotAllocated var)
-      else None in
-  if checkGhosts
-  then if vnth (rsGhostAllocs st) var is Some reg
-       then check (rsGhostRegs st) reg
-       else go
-  else go.
-
-Definition checkLiveness st : seq 'I_maxVar -> seq AllocError :=
-  flip (forFold [::]) $ fun acc var =>
-    if checkAlloc' st var None false false is Some err
-    then err :: acc
-    else acc.
-
-Definition liveRegisters st : seq 'I_maxVar -> seq 'I_maxReg :=
-  flip (forFold [::]) $ fun acc var =>
-    if vnth (rsAllocs st) var is Some reg
-    then reg :: acc
-    else acc.
-
-Definition clearGhost (reg : 'I_maxReg) (var : 'I_maxVar)
-  (ghostRegs   : Vec (option 'I_maxVar) maxReg)
-  (ghostAllocs : Vec (option 'I_maxReg) maxVar) :
-  (Vec (option 'I_maxVar) maxReg * Vec (option 'I_maxReg) maxVar) :=
-  (if vnth ghostAllocs var is Some r
-   then vreplace ghostRegs r None
-   else ghostRegs,
-   if vnth ghostRegs reg is Some v
-   then vreplace ghostAllocs v None
-   else ghostAllocs).
-
 Inductive RegState : RegStateDesc -> Prop :=
   | StartState : RegState newRegStateDesc
 
-  | AllocRegS st r v :
-    vnth (rsRegs   st) r == None ->
-    vnth (rsAllocs st) v == None ->
+  | ReserveRegS st r v :
+    vnth (rsAllocs st) r ^_ reservation == None ->
     RegState
-      {| rsRegs        := vreplace (rsRegs   st) r (Some v)
-       ; rsAllocs      := vreplace (rsAllocs st) v (Some r)
-       ; rsGhostRegs   := rsGhostRegs   st
-       ; rsGhostAllocs := vreplace (rsGhostAllocs st) v None
-       ; rsStack       := rsStack st
+      {| rsAllocs := vmodify (rsAllocs st) r (reservation .~ Some v)
+       ; rsStack  := rsStack st
        |}
 
-  | FreeRegS st r v :
-    vnth (rsRegs   st) r == Some v ->
-    vnth (rsAllocs st) v == Some r ->
-    let: (gregs, gallocs) :=
-       clearGhost r v (rsGhostRegs st) (rsGhostAllocs st) in
+  | ReleaseRegS st r v :
+    vnth (rsAllocs st) r ^_ reservation == Some v ->
     RegState
-      {| rsRegs        := vreplace (rsRegs   st) r None
-       ; rsAllocs      := vreplace (rsAllocs st) v None
-       ; rsGhostRegs   := vreplace gregs r (Some v)
-       ; rsGhostAllocs := vreplace gallocs v (Some r)
-       ; rsStack       := rsStack st
+      {| rsAllocs := vmodify (rsAllocs st) r (reservation .~ None)
+       ; rsStack  := rsStack st
        |}
 
-  | ClearGhostsS st :
+  | AssignRegS st r v :
+    vnth (rsAllocs st) r ^_ reservation == Some v ->
     RegState
-      {| rsRegs        := rsRegs st
-       ; rsAllocs      := rsAllocs st
-       ; rsGhostRegs   := vconst None
-       ; rsGhostAllocs := vconst None
-       ; rsStack       := rsStack st
+      {| rsAllocs := vmodify (rsAllocs st) r (residency .~ Some v)
+       ; rsStack  := rsStack st
+       |}
+
+  | ClearRegS st r v :
+    vnth (rsAllocs st) r ^_ residency == Some v ->
+    RegState
+      {| rsAllocs := vmodify (rsAllocs st) r (residency .~ None)
+       ; rsStack  := rsStack st
        |}
 
   | AllocStackS st v :
-    vnth (rsAllocs st) v == None ->
-    vnth (rsStack  st) v == false ->
+    ~~ IntSet_member v (rsStack st) ->
     RegState
-      {| rsRegs        := rsRegs st
-       ; rsAllocs      := rsAllocs st
-       ; rsGhostRegs   := rsGhostRegs st
-       ; rsGhostAllocs := rsGhostAllocs st
-       ; rsStack       := vreplace (rsStack st) v true
+      {| rsAllocs := rsAllocs st
+       ; rsStack  := IntSet_insert v (rsStack st)
        |}
 
   | FreeStackS st v :
-    vnth (rsAllocs st) v == None ->
-    vnth (rsStack  st) v == true ->
+    IntSet_member v (rsStack st) ->
     RegState
-      {| rsRegs        := rsRegs st
-       ; rsAllocs      := rsAllocs st
-       ; rsGhostRegs   := rsGhostRegs st
-       ; rsGhostAllocs := rsGhostAllocs st
-       ; rsStack       := vreplace (rsStack st) v false
+      {| rsAllocs := rsAllocs st
+       ; rsStack  := IntSet_delete v (rsStack st)
        |}.
+
+Definition RegStateSig := { rd : RegStateDesc | RegState rd }.
 
 Definition getRegStateDesc `(st : RegState rd) := rd.
 Arguments getRegStateDesc [rd] st /.
@@ -201,15 +112,11 @@ Arguments packRegState [rd] st /.
 
 Variable A : Type.
 
-Definition BlockExitAllocations :=
-  IntMap (seq (('I_maxVar + 'I_maxVar) * 'I_maxReg)).
-
 Record VerifiedSig := {
   verDesc   : RegStateDesc;
   verState  : RegState verDesc;
-  (* [verBlocks] gives the final allocation state for any blocks; it only
-     contains mappings for variables listed in a block's "live out" set. *)
-  verBlocks : BlockExitAllocations;
+  (* [verBlocks] gives the final allocation state for every handled block *)
+  verBlocks : IntMap RegStateSig;
   verMoves  : IntMap (seq (@ResolvingMove maxReg));
   verErrors : IntMap (seq AllocError);
   verExt    : A
@@ -237,7 +144,8 @@ Definition _verState :
      ; verExt    := verExt s
      |}) (f (verDesc s; verState s)).
 
-Definition _verBlocks : Lens' VerifiedSig BlockExitAllocations := fun _ _ f s =>
+Definition _verBlocks : Lens' VerifiedSig (IntMap RegStateSig) :=
+  fun _ _ f s =>
   fmap (fun x =>
     {| verDesc   := verDesc s
      ; verState  := verState s
@@ -291,155 +199,101 @@ Definition errorT (err : AllocError) : Verified unit :=
 
 Variable useVerifier : UseVerifier.
 
-Definition checkAlloc (var : 'I_maxVar) (reg : 'I_maxReg) (checkGhosts : bool) :
-  Verified unit :=
-  st <-- use _verDesc ;;
-  if checkAlloc' st var (Some reg)
-                 (if useVerifier is VerifyEnabled
-                  then true else false) checkGhosts is Some err
-  then errorT err
-  else pure tt.
-
 Definition addMove (mv : @ResolvingMove maxReg) : Verified unit :=
   _verMoves %= IntMap_alter
     (fun mxs => @Some _ $ if mxs is Some xs
                           then rcons xs mv
                           else [:: mv]) pc.
 
-Definition allocReg (reg : 'I_maxReg) (var : 'I_maxVar) : Verified unit :=
+Definition reserveReg (reg : PhysReg) (var : VarId) : Verified unit :=
   addMove $ AllocReg var reg ;;
   st <-- use _verDesc ;;
-  decide (vnth (rsRegs st) reg == None)
-    (fun H1 =>
-       decide (vnth (rsAllocs st) var == None)
-         (fun H2 => _verState .= packRegState (AllocRegS H1 H2))
-         (fun _  =>
-            if vnth (rsAllocs st) var is Some r
-            then errorT $ AllocVarAllocatedToDifferentReg var r reg
-            else pure tt))
-    (fun _  =>
-       if vnth (rsRegs st) reg is Some v
-       then
-         when (v != var) $
-           errorT $ AllocRegAllocatedToDifferentVar reg v var
-       else pure tt).
+  if prop (vnth (rsAllocs st) reg ^_ reservation == None) is Some H
+  then _verState .= packRegState (ReserveRegS var H)
+  else if vnth (rsAllocs st) reg ^_ reservation is Some v
+       then when (v != var) $
+              errorT $ RegAlreadyReservedToVar reg v var
+       else pure tt.
 
-Definition freeReg (reg : 'I_maxReg) (var : 'I_maxVar) : Verified unit :=
+Definition isReserved (reg : PhysReg) (var : VarId) : Verified bool :=
+  st <-- use _verDesc ;;
+  pure (vnth (rsAllocs st) reg ^_ reservation == Some var).
+
+Definition checkReservation (reg : PhysReg) (var : VarId) : Verified unit :=
+  st <-- use _verDesc ;;
+  b  <-- isReserved reg var ;;
+  if b
+  then pure tt
+  else errorT $ VarNotReservedForReg var reg.
+
+Definition releaseReg (reg : PhysReg) (var : VarId) : Verified unit :=
   addMove $ FreeReg reg var ;;
   st <-- use _verDesc ;;
-  decide (vnth (rsRegs st) reg == Some var)
-    (fun H1 =>
-       decide (vnth (rsAllocs st) var == Some reg)
-         (fun H2 => _verState .= packRegState (FreeRegS H1 H2))
-         (fun _  =>
-            if vnth (rsAllocs st) var is Some r
-            then errorT $ FreeVarAllocatedToDifferentReg var r reg
-            else errorT $ FreeUnallocatedVar var))
-    (fun _  => errorT $ FreeRegNotAllocatedToVar reg var).
+  if prop (vnth (rsAllocs st) reg ^_ reservation == Some var) is Some H
+  then _verState .= packRegState (ReleaseRegS H)
+  else errorT $ VarNotReservedForReg var reg.
+
+Definition assignReg (reg : PhysReg) (var : VarId) : Verified unit :=
+  st <-- use _verDesc ;;
+  if prop (vnth (rsAllocs st) reg ^_ reservation == Some var) is Some H
+  then _verState .= packRegState (AssignRegS H)
+  else errorT $ VarNotReservedForReg reg var.
+
+Definition isResident (reg : PhysReg) (var : VarId) : Verified bool :=
+  st <-- use _verDesc ;;
+  pure (vnth (rsAllocs st) reg ^_ residency == Some var).
+
+Definition checkResidency (reg : PhysReg) (var : VarId) : Verified unit :=
+  st <-- use _verDesc ;;
+  b  <-- isResident reg var ;;
+  if b
+  then pure tt
+  else errorT $ VarNotResidentForReg var reg.
+
+Definition clearReg (reg : PhysReg) (var : VarId) : Verified unit :=
+  st <-- use _verDesc ;;
+  if prop (vnth (rsAllocs st) reg ^_ residency == Some var) is Some H
+  then _verState .= packRegState (ClearRegS H)
+  else errorT $ VarNotResidentForReg var reg.
 
 (* Definition allocStack (v : 'I_maxVar) : Verified unit := pure tt. *)
 
 (* Definition freeStack (v : 'I_maxVar) : Verified unit := pure tt. *)
 
-Lemma size_is0 : forall a (l : seq a), l = nil -> size l == 0.
-Proof. move=> a. by case. Qed.
-
-Definition checkVar (vid : VarId) : Verified 'I_maxVar :=
-  if prop (vid < maxVar) is Some H
-  then pure $ Ordinal H
-  else
-    errorT $ VarId_OutOfBounds vid maxVar ;;
-    pure $ Ordinal variables_exist.
+Definition checkLiveness (vars : IntSet) : Verified unit :=
+  st <-- use _verDesc ;;
+  forM_ (IntSet_toList vars) $ fun var =>
+    unless (vfoldl_with_index (fun reg b p =>
+      b || if p ^_ residency is Some var then true else false)
+                              false (rsAllocs st)) $
+      errorT $ VarNotResident var.
 
 Definition verifyBlockBegin (bid : nat) (liveIns : IntSet) (loops : LoopState) :
   Verified unit :=
   if useVerifier is VerifyDisabled then pure tt else
-  if IntMap_lookup bid (forwardBranches loops) is Some fwds
-  then
-    forFoldM true (IntSet_toList fwds) (fun isFirst pred =>
-      exits <-- use _verBlocks ;;
-      (if IntMap_lookup pred exits isn't Some allocs
+  (if IntMap_lookup bid (forwardBranches loops) is Some fwds
+   then
+     forM_ (IntSet_toList fwds) (fun pred =>
+       exits <-- use _verBlocks ;;
+       if IntMap_lookup pred exits isn't Some allocs
        then errorT $ UnknownPredecessorBlock bid pred
-       (* else forM_ (IntSet_toList liveIns) $ fun vid => *)
-       (*   var <-- checkVar vid ;; *)
-       (*   if maybeLookup allocs (inr var) is Some reg *)
-       (*   then allocReg reg var *)
-       (*   else *)
-       (*     if maybeLookup allocs (inl var) is Some reg *)
-       (*     then allocReg reg var ;; *)
-       (*          freeReg reg var *)
-       (*     else errorT $ VarWithoutAllocation vid *)
-       else
-         forM_ (IntSet_toList liveIns) (fun vid =>
-           var <-- checkVar vid ;;
-           if maybeLookup allocs (inr var) is Some reg
-           then pure tt
-           else
-             if maybeLookup allocs (inl var) is Some reg
-             then pure tt
-             else errorT $ VarWithoutAllocation vid) ;;
-         when isFirst $
-           forM_ allocs $ fun z =>
-             match z with
-             | (inl var, reg) => allocReg reg var ;;
-                                 freeReg reg var
-             | (inr var, reg) => allocReg reg var
-             end) ;;
-      pure false) ;;
-    pure tt
-  else
-    if IntSet_size liveIns == 0
-    then pure tt
-    else
-      if useVerifier is VerifyEnabledUnitializedOK
-      then pure tt
-      else errorT $ BlockWithoutPredecessors bid.
+       else _verState .= allocs)
+   else
+     when (IntSet_size liveIns > 0) $
+       errorT $ BlockWithoutPredecessors bid) ;;
+  checkLiveness liveIns.
 
 Definition verifyBlockEnd (bid : nat) (liveOuts : IntSet) : Verified unit :=
   if useVerifier is VerifyDisabled then pure tt else
-  st <-- use _verDesc ;;
+  (* Check to ensure that all "live out" variables are resident in registers
+     at the end of the block. *)
+  checkLiveness liveOuts ;;
 
-  let allocs := vfoldl_with_index
-    (fun var acc mreg =>
-       if mreg is Some reg
-       then (inr var, reg) :: acc
-       else acc) [::] (rsAllocs st) in
+  (* Clear out all known allocations, saving them for this block. *)
+  allocs <-- use _verState ;;
+  _verState .= packRegState StartState ;;
 
-  let allocs' := vfoldl_with_index
-    (fun var acc mreg =>
-       if mreg is Some reg
-       then if maybeLookup acc (inr var) is None
-            then if maybeValueLookup acc reg is None
-                 then (inl var, reg) :: acc
-                 else acc
-            else acc
-       else acc) allocs (rsGhostAllocs st) in
-
-  _verBlocks %= IntMap_insert bid allocs' ;;
-
-  decide (all (ltn ^~ maxVar) (IntSet_toList liveOuts))
-    (fun L =>
-       let vars := IntSet_to_seq_fin L in
-       st <-- use _verDesc ;;
-       if checkLiveness st vars is e :: es
-       then errorsT $ ErrorAtBlockEnd bid :: e :: es
-       else pure tt)
-    (fun _ =>
-       forM_ (IntSet_toList liveOuts) $ fun var =>
-         when (maxVar <= var) $
-           errorT $ VarId_OutOfBounds var maxVar) ;;
-
-  (* Clear out all known allocations *)
-  _verState .= packRegState StartState.
-
-(*
-Definition replaceReg (reg : 'I_maxReg) (var : 'I_maxVar) : Verified unit :=
-  st <-- use _verDesc ;;
-  (if vnth (rsRegs st) reg is Some v
-   then freeReg reg v
-   else pure tt) ;;
-  allocReg reg var.
-*)
+  _verBlocks %= IntMap_insert bid allocs.
 
 Definition verifyApplyAllocs (op : opType1) (allocs : seq (VarId * PhysReg)) :
   Verified (seq opType2) :=
@@ -453,19 +307,25 @@ Definition verifyApplyAllocs (op : opType1) (allocs : seq (VarId * PhysReg)) :
          (* Direct register references are mostly left alone; we just check to
             make sure that it's not overwriting a variable in a register. *)
          st <-- use _verDesc ;;
-         if vnth (rsRegs st) reg is Some v
-         then errorT $ RegAlreadyAllocatedTo reg v
-         else pure tt
-
-       | inr vid =>
-         if maybeLookup allocs vid isn't Some reg
-         then errorT $ VarWithoutAllocation vid
+         if varKind ref is Input
+         then
+           if vnth (rsAllocs st) reg is (Some v, _)
+           then errorT $ PhysRegAlreadyResidentForVar reg v
+           else pure tt
          else
-           var <-- checkVar vid ;;
+           if vnth (rsAllocs st) reg is (_, Some v)
+           then errorT $ PhysRegAlreadyReservedForVar reg v
+           else pure tt
+
+       | inr var =>
+         if maybeLookup allocs var isn't Some reg
+         then errorT $ VarNotAllocated var
+         else
            match varKind ref with
-           | Input  => checkAlloc var reg true
-           | Temp   => pure tt         (* jww (2015-07-04): What to do here? *)
-           | Output => checkAlloc var reg false
+           | Input  => checkResidency reg var
+           | Temp   => checkReservation reg var
+           | Output => checkReservation reg var ;;
+                       assignReg reg var
            end
        end)
    else pure tt) ;;
@@ -480,74 +340,51 @@ Definition verifyResolutions (moves : seq (@ResGraphEdge maxReg)) :
     st <-- use _verDesc ;;
     match resMove mv with
     | Move fromReg fromVar toReg =>
-      if vnth (rsRegs st) fromReg isn't Some fromVar
-      then
-        errorT $ MoveRegNotAllocated fromReg toReg ;;
+      checkResidency fromReg fromVar ;;
+      unless (fromReg == toReg) $
+        releaseReg fromReg fromVar ;;
+        reserveReg toReg fromVar ;;
         addMove (resMove mv) ;;
-        pure acc
-      else
-        if fromReg == toReg
-        then pure acc
-        else
-          freeReg fromReg fromVar ;;
-          allocReg toReg fromVar ;;
-          addMove (resMove mv) ;;
-          when (resGhost mv) (freeReg toReg fromVar) ;;
-          pure $ resMove mv :: acc
+        assignReg toReg fromVar ;;
+        when (resGhost mv) (releaseReg toReg fromVar) ;;
+        pure $ resMove mv :: acc
 
     | Swap fromReg fromVar toReg toVar =>
-      if vnth (rsRegs st) fromReg isn't Some fromVar
-      then
-        errorT $ SwapRegNotAllocated fromReg toReg ;;
-        addMove (resMove mv) ;;
-        pure acc
-      else
-        if vnth (rsRegs st) toReg isn't Some toVar
-        then
-          errorT $ SwapRegNotAllocated toReg fromReg ;;
-          addMove (resMove mv) ;;
-          pure acc
-        else
-          if fromVar != toVar
-          then checkAlloc toVar toReg false ;;
-               checkAlloc fromVar fromReg false ;;
-               addMove (resMove mv) ;;
-               pure $ resMove mv :: acc
-          else pure acc
+      checkResidency fromReg fromVar ;;
+      checkResidency toReg toVar ;;
+      releaseReg fromReg fromVar ;;
+      releaseReg toReg toVar ;;
+      addMove (resMove mv) ;;
+      reserveReg fromReg toVar ;;
+      reserveReg toReg fromVar ;;
+      assignReg fromReg toVar ;;
+      assignReg toReg fromVar ;;
+      pure $ resMove mv :: acc
 
     | Spill fromReg toSpillSlot =>
-      if vnth (rsRegs st) fromReg isn't Some fromVar
-      then
-        errorT $ SpillRegNotAllocated fromReg toSpillSlot ;;
-        addMove (resMove mv) ;;
-        pure acc
-      else
-        stackVar <-- checkVar toSpillSlot ;;
-        if fromVar != stackVar
-        then
-          errorT $ SpillToWrongSlot fromReg fromVar toSpillSlot ;;
-          addMove (resMove mv) ;;
-          pure acc
-        else
-          addMove (resMove mv) ;;
-          freeReg fromReg fromVar ;;
-          pure $ resMove mv :: acc
+      releaseReg fromReg toSpillSlot ;;
+      check <-- isResident fromReg toSpillSlot ;;
+      if check
+      then addMove (resMove mv) ;;
+           pure $ resMove mv :: acc
+      else pure acc
 
     | Restore fromSpillSlot toReg =>
-      stackVar <-- checkVar fromSpillSlot ;;
-      allocReg toReg stackVar ;;
+      reserveReg toReg fromSpillSlot ;;
       addMove (resMove mv) ;;
-      when (resGhost mv) (freeReg toReg stackVar) ;;
+      assignReg toReg fromSpillSlot ;;
+      when (resGhost mv)
+        (releaseReg toReg fromSpillSlot) ;;
       pure $ resMove mv :: acc
 
     | AllocReg toVar toReg =>
-      var <-- checkVar toVar ;;
-      allocReg toReg var ;;
-      when (resGhost mv) (freeReg toReg var) ;;
+      reserveReg toReg toVar ;;
+      when (resGhost mv)
+        (releaseReg toReg toVar) ;;
       pure acc
 
     | FreeReg fromReg fromVar =>
-      checkVar fromVar >>= freeReg fromReg ;;
+      releaseReg fromReg fromVar ;;
       pure acc
 
     (* | AllocStack toVar => pure acc *)
@@ -563,16 +400,16 @@ Include LensLaws.
 Variable a b : Type.
 Variable P : a -> Prop.
 
-(* Program Instance Lens__verDesc : GetterLaws (@_verDesc maxReg maxVar a). *)
-Program Instance Lens__verState : LensLaws (@_verState maxReg maxVar a).
+(* Program Instance Lens__verDesc : GetterLaws (@_verDesc maxReg a). *)
+Program Instance Lens__verState : LensLaws (@_verState maxReg a).
 Obligation 2. by case: x. Qed.
-Program Instance Lens__verBlocks : LensLaws (@_verBlocks maxReg maxVar a).
+Program Instance Lens__verBlocks : LensLaws (@_verBlocks maxReg a).
 Obligation 2. by case: x. Qed.
-Program Instance Lens__verMoves : LensLaws (@_verMoves maxReg maxVar a).
+Program Instance Lens__verMoves : LensLaws (@_verMoves maxReg a).
 Obligation 2. by case: x. Qed.
-Program Instance Lens__verErrors : LensLaws (@_verErrors maxReg maxVar a).
+Program Instance Lens__verErrors : LensLaws (@_verErrors maxReg a).
 Obligation 2. by case: x. Qed.
-Program Instance Lens__verExt : LensLaws (@_verExt maxReg maxVar a).
+Program Instance Lens__verExt : LensLaws (@_verExt maxReg a).
 Obligation 2. by case: x. Qed.
 
 End VerifyLensLaws.
